Otway-Rees: attempt to model msg2 interception attack (verification fails)
It seems like the corruption of a malicious principal eve invalidates the trace.
Hence, this commit does not contain a complete/executable version of the attack.
The attack implementation will be worked on as soon as a solution for this problem
has been found.

otway-rees/OYRS.Debug.fst
@@ -11,6 +11,7 @@ open LabeledPKI
 open AttackerAPI
 open OYRS.Sessions
 open OYRS.Protocol
+open OYRS.Attacker
 
 
 val benign_attacker:
@@ -36,11 +37,59 @@ let benign_attacker () =
   let msg4_idx = responder_send_msg_4 b msg3_idx b_si in
   initiator_recv_msg_4 a msg4_idx a_si
 
+val intercept_msg_2_attacker:
+  unit ->
+  LCrypto unit (pki oyrs_preds)
+  (requires fun _ -> True)
+  (ensures fun _ _ _ -> True)
+
+let intercept_msg_2_attacker () =
+  let a:principal = "initiator" in
+  let b:principal = "responder" in
+  let srv:principal = "server" in
+  let eve:principal = "eve" in
+
+  let ts0 = global_timestamp () in
+  let ((|t_as,us_as,k_as|), a_si) = initiator_init a srv b in
+  let ((|t_bs,us_bs,k_bs|), b_si) = responder_init b srv in
+  install_sk_at_auth_server #t_as #us_as srv a k_as;
+  let ts1 = global_timestamp () in
+  install_sk_at_auth_server #t_bs #us_bs srv b k_bs;
+  let ts2 = global_timestamp () in
+
+  let pr = (pki oyrs_preds) in
+  let tr = get () in
+  assert(valid_trace pr tr);
+
+  let ts_corr_eve = AttackerAPI.compromise eve 0 0 in
+
+  let ts3 = global_timestamp () in
+  assert(was_corrupted_before ts3 eve 0 0);
+  assert(later_than ts3 ts_corr_eve);
+
+  let tr = get () in
+  assert(valid_trace pr tr);
+
+  //let msg1_idx = initiator_send_msg_1 a a_si in
+  //let msg2_idx = responder_send_msg_2 b msg1_idx b_si in
+  // third message from auth server is discarded
+  //let msg3_idx = attacker_intercept_msg_2 eve srv b msg2_idx in
+  //let msg4_idx = responder_send_msg_4 b msg3_idx b_si in
+  //initiator_recv_msg_4 a msg4_idx a_si;
+  ()
+
 let benign () : LCrypto unit (pki oyrs_preds)
   (requires (fun _ -> True)) (ensures (fun _ _ _ -> True))
 = print_string "start\n";
   let t0 = get() in
   let x = benign_attacker () in
+  print_trace ()
+
+let intercept_msg_2 () : LCrypto unit (pki oyrs_preds)
+  (requires (fun _ -> True)) (ensures (fun _ _ _ -> True))
+= print_string "start\n";
+  let t0 = get() in
+  let x = intercept_msg_2_attacker () in
   print_trace ()
 
 let main =
@@ -55,3 +104,10 @@ let main =
   | Error s -> IO.print_string ("ERROR: "^s^"\n")
   | Success _ -> IO.print_string "PROTOCOL RUN: Successful execution of Otway-Rees protocol.\n");
   IO.print_string "Finished Benign Attacker:\n"
+  IO.print_string "Starting Intercept Msg2 Attacker:\n";
+  assume(valid_trace (pki oyrs_preds) t0);
+  let r,t1 = (reify (intercept_msg_2 ()) t0) in
+  (match r with
+  | Error s -> IO.print_string ("ERROR: "^s^"\n")
+  | Success _ -> IO.print_string "PROTOCOL RUN: Successful execution of Otway-Rees protocol.\n");
+  IO.print_string "Finished Intercept Msg2 Attacker:\n"
