otway-rees/OYRS.Attacker.fst
@@ -1,0 +1,56 @@
+module OYRS.Attacker
+
+
+open SecrecyLabels
+open CryptoEffect
+open CryptoLib
+open GlobalRuntimeLib
+open LabeledRuntimeAPI
+
+module S = OYRS.Sessions
+module L = LabeledPKI
+module A = AttackerAPI
+
+
+let attacker_intercept_msg_2 (eve srv bob:principal) (msg2_idx:nat) :
+  Crypto timestamp
+         (requires (fun t0 -> msg2_idx < trace_len t0))
+         (ensures (fun t0 n t1 ->
+         match n with
+         | Error _ -> t0 == t1
+         | Success n ->
+           A.attacker_modifies_trace t0 t1 /\
+           trace_len t1 = trace_len t0 + 1 /\
+           later_than (trace_len t1) (trace_len t0) /\
+           n = trace_len t0))
+= // receive and parse second message
+  let (|t_m2,ser_msg2|) = A.receive_i msg2_idx eve in
+
+  match
+    A.split ser_msg2 `bind` (fun (tag_bytes, rest) ->
+    A.pub_bytes_to_string tag_bytes `bind` (fun tag ->
+    match tag with
+    | "msg2" ->
+      A.split rest `bind` (fun (c, rest) ->
+      A.split rest `bind` (fun (_, rest) ->
+      A.split rest `bind` (fun (_, rest) ->
+      A.split rest `bind` (fun (ev_a, ev_b) ->
+      Success (|c,ev_a,ev_b|)))))
+    | t -> Error ("attacker_intercept_m2: wrong message: " ^ t)
+    ))
+  with
+  | Success (|c,ev_a,ev_b|) ->
+    // create and send malicious third message
+    let now = global_timestamp () in
+    let msg3_tag = A.pub_bytes_later 0 now (A.string_to_pub_bytes "msg3") in
+    let c = A.pub_bytes_later t_m2 now c in
+    (* ev_a and ev_b will be interpreted as (nonce, key) where the key is the
+    concatenation (c, a, b) in reality. c, a and b are all public. Thus, the
+    attacker is in posession of the conversation key that is supposed to be
+    secret. *)
+    let ev_a = A.pub_bytes_later t_m2 now ev_a in
+    let ev_b = A.pub_bytes_later t_m2 now ev_b in
+    let ser_msg3 = A.concat msg3_tag (A.concat c (A.concat ev_a ev_b)) in
+
+    A.send #now srv bob ser_msg3
+  | Error e -> error e
